stanfrontend/CStan.v
@@ -343,3 +343,4 @@ Require Import Linking.
 
 Instance L: Linker CStan.program.
 Admitted.
+
